veric/mpred.v
@@ -148,6 +148,17 @@ Definition const_super_non_expansive: forall (T: Type) P,
   @super_non_expansive (ConstType T) P :=
   fun _ _ _ _ _ _ => eq_refl.
 
+Definition AssertListTT (A: TypeTree): TypeTree :=
+  ArrowType A (ArrowType (ConstType environ) (ListType Mpred)).
+
+Definition super_non_expansive_list {A: TypeTree}
+  (P: forall ts, dependent_type_functor_rec ts (AssertListTT A) mpred): Prop :=
+  forall n ts
+    (x: functors.MixVariantFunctor._functor
+                         (rmaps.dependent_type_functor_rec ts A) mpred)
+    (rho: environ),
+  Forall2 (fun a b => approx n a = approx n b) (P ts x rho) (P ts (fmap _ (approx n) (approx n) x) rho).
+
 (*Potential alternative that does not use Ctypes
 Inductive funspec :=
    mk_funspec: AST.signature -> forall (A: TypeTree)
